## für $n \in \mathbb{N}$
$$
(x+y)^n =\sum^{n}_{i=0} {^nC_i} · x^{n-1}y^i
$$
$$
\begin{align}
{^nC_i}=\frac{n!}{(n-i)!·i!}
\end{align}
$$
## Für Rationale Zahlen

*Wir gehen davon aus das |a|>|b|*

$$
\begin{align}
(a+b)^n &= \left\{a\left(1+\frac{b}{a}\right)\right\}^n\\
&=a^n\left(1+\frac{b}{a}\right)^n\\
&=a^n(1+x)^n \;\;\;\;\;\;\;\; where \; |n|<1
\end{align}
$$

$$
\begin{align}
&(1+x)^n=1+nx+\frac{n(n-1)}{2!}x^2+\frac{n(n-1)(n-2)}{3!}x^3+...\\
&...+\frac{n(n-1)(n-2)......(n-r+1)}{r!}x^r...\infty
\end{align}
$$
