
## Negationsregel

$$
\begin{align}
\neg(\forall x :p(x)) \equiv \exists x : \neg p(x)
\end{align}
$$
$$
\begin{align}
\neg(\exists x : p(x)) \equiv \forall x : \neg p(x)
\end{align}
$$
$$
\begin{align}
\neg(\forall x \exists y : G(x,y))
& \equiv    \exists x : \neg (\exists y : G(x,y)) \\
& \equiv \exists x \forall y : \neg G(x,y) 
\end{align}
$$


## Ausklammerregeln

$$
\begin{align}
(\forall x : F(x)) \wedge (\forall x : G(x)) \equiv \forall x (F(x) \vee G(x)) 
\end{align}
$$
$$
(\exists x : F(x)) \vee (\exists x : G(x)) \equiv \exists x (F(x) \wedge G(x))
$$
## Vertauschungsregeln

$$
\forall x \forall y : F(x,y) \equiv \forall y \forall x : F(x,y) 
$$
$$
\exists x \exists y : F(x,y) \equiv \exists y \exists x : F(x,y)
$$
