![[Pasted image 20240410201242.png]]
## Steigung
![[Pasted image 20240410201217.png]]
$$
\begin{align}
m =: f'(x) := \lim_{\triangle x \rightarrow 0} \frac{\triangle y}{\triangle x} &= \lim_{\triangle x \rightarrow 0} \frac{f(x+\triangle x) - f(x)}{\triangle x} \\
&= \lim_{\triangle x \rightarrow 0} \frac{(x + \triangle x)^2 - x^2}{\triangle x} \\
&= \lim_{\triangle x \rightarrow 0} \frac{x^2 + 2x \triangle x + \triangle x^2 - x^2}{\triangle x} \\
&= \lim_{\triangle x \rightarrow 0} \frac{2x \triangle x + \triangle x^2}{\triangle x} \\
&= \lim_{\triangle x \rightarrow 0} 2x + \triangle x \\
&= 2x
\end{align}
$$
## Leibniz
$$
\begin{align}
\triangle &= (endliche) \ Differenz \\
d &= (undendlich \ kleine) \ Differenz \\
f'(x) &= \lim_{\triangle x \rightarrow 0} \frac{\triangle y}{\triangle x} = \frac{dy}{dx} \rightarrow Leibniz \ Schreibweise \\
\frac{\triangle y}{\triangle x} &= Differenzquotient \\
\frac{dy}{dx} &= Differentialquotient \\
dx &= Differntialoperator \rightarrow Funktion, \ die \ auf \ Funktionen \ wirkt \\
\end{align}
$$
### Beispiel

$$
\begin{align}
f'(x) &= \frac{df}{dx} \\
f''(x) &= \frac{d}{dx} \left( \frac{d}{dx}f \right) \\
&= \left( \frac{d}{dx} \frac{d}{dx} f\right) \\
&= \left( \frac{d}{dx} \right)^2 f \\
&= \frac{d^2}{dx^2}f \\
&= \frac{d^2f}{dx^2}
\end{align}
$$

# Vorsicht!!!!
$$
\begin{align}
\frac{df^2}{dx^2} &= [f'(x)]^2 \\
\frac{df^2}{dx^2} &= \left( \frac{df}{dx} \right)^2 = (f'(x))^2
\end{align}
$$

## Regeln
- **elementare Ableitungen**
$$
\begin{align}
&f \ \ \ \ f' \\
&x^n \rightarrow x^{n-1} \\
&e^x \rightarrow e^x \\
&\ln x = \frac{1}{x} \\
& \sin x \rightarrow \cos x \\
& \cos x \rightarrow - \sin x
\end{align}
$$
- **Ableitungen sind linear**
$$
\begin{align}
\frac{d}{dx} (f + g) &= \frac{d}{dx}f + \frac{d}{dx} g \\
\frac{d}{dx}(c · f) &= c · \frac{d}{dx} f
\end{align}
$$
- **Ableitungsregeln**
$$
\begin{align}
(f·g)' &= f' · g + f · g' \\
\left[\frac{f}{g}\right] &= \frac{g · f' - f · g'}{g^2} \ Quotientenregel \\
f(u(x)) &= f'(u) · u'(x)
\end{align}
$$